integrate lennart's HMAC pure lemmas (2 not working: mkArgZ and spec_sha dependency)

HMAC_functional_prog_Z.v
@@ -21,16 +21,12 @@ Module Type HMAC_Module.
 End HMAC_Module.
 
 Module HMAC_FUN (HF:HASH_FUNCTION)  <: HMAC_Module.
-Fixpoint Nlist {A} (i:A) n: list A:=
-  match n with O => nil
-  | S m => i :: Nlist i m
-  end.
 
-Definition sixtyfour {A} (i:A): list A:= Nlist i HF.BlockSize.
+Definition sixtyfour {A} (i:A): list A:= list_repeat HF.BlockSize i.
 
 (*Reading rfc4231 reveals that padding happens on the right*)
 Definition zeroPad (k: list Z) : list Z :=
-  k ++ Nlist Z0 (HF.BlockSize-length k).
+  k ++ list_repeat (HF.BlockSize-length k) Z0.
 
 Definition mkKey (l:list Z) : list Z :=
   if Z.gtb (Zlength l) (Z.of_nat HF.BlockSize)
@@ -101,6 +97,7 @@ Definition check password text digest :=
 
 (*a random example, solution obtained via 
   http://www.freeformatter.com/hmac-generator.html#ad-output*)
+
 Goal check "bb" "aa"
       "c1201d3dccfb84c069771d07b3eda4dc26e5b34a4d8634b2bba84fb54d11e265". 
 vm_compute. reflexivity. Qed.
